Simplify CSE, Constprop, Deadcode.

backend/CSEproof.v
@@ -825,7 +825,6 @@ Hypothesis TRANSF:
     prog tprog.
 Let ge := Genv.globalenv prog.
 Let tge := Genv.globalenv tprog.
-Let rm := romem_for_program prog.
 
 Inductive match_fundef prog: forall (fd fd':fundef), Prop :=
 | match_fundef_transl fd fd' sprog
@@ -959,9 +958,10 @@ Inductive match_stackframes: list stackframe -> list stackframe -> Prop :=
   | match_stackframes_nil:
       match_stackframes nil nil
   | match_stackframes_cons:
-      forall res sp pc rs f approx s rs' s' sprog
+      forall res sp pc rs f approx s rs' s' sprog rm
+           (ANALYZE: analyze f (vanalyze rm f) = Some approx)
+           (RM: rm = romem_for_program sprog)
            (SPROG: program_linksub Language_RTL sprog prog)
-           (ANALYZE: analyze f (vanalyze (romem_for_program sprog) f) = Some approx)
            (SAT: forall v m, exists valu, numbering_holds valu ge sp (rs#res <- v) m approx!!pc)
            (RLD: regs_lessdef rs rs')
            (STACKS: match_stackframes s s'),
@@ -987,9 +987,10 @@ Inductive match_identical_states: state -> state -> Prop :=
 
 Inductive match_states: state -> state -> Prop :=
   | match_states_intro:
-      forall s sp pc rs m s' rs' m' f approx sprog
+      forall s sp pc rs m s' rs' m' f approx sprog rm
+             (ANALYZE: analyze f (vanalyze rm f) = Some approx)
+             (RM: rm = romem_for_program sprog)
              (SPROG: program_linksub Language_RTL sprog prog)
-             (ANALYZE: analyze f (vanalyze (romem_for_program sprog) f) = Some approx)
              (SAT: exists valu, numbering_holds valu ge sp rs m approx!!pc)
              (RLD: regs_lessdef rs rs')
              (MEXT: Mem.extends m m')
@@ -1374,7 +1375,7 @@ Lemma CSE_sepcomp_rel
       (Htrans: CSE.transf_program rtlprog1 = OK rtlprog2 \/ rtlprog1 = rtlprog2):
   @sepcomp_rel
     Language.Language_RTL Language.Language_RTL
-    (fun p f tf => CSE.transf_function (ValueAnalysis.romem_for_program p) f = OK tf \/ f = tf)
+    (fun p f tf => CSE.transf_function (romem_for_program p) f = OK tf \/ f = tf)
     (fun p ef tef => (fun _ ef => OK ef) p ef = OK tef)
     (@OK _)
     rtlprog1 rtlprog2.
